Before removing DAnd

Regex/Termination.lean
@@ -18,77 +18,77 @@ macro "termination" : tactic =>
 end Tactic
 
 /-- A regex that always terminates, regardless of inputs to `matchPartial` -/
-def AlwaysTerminates (r : Regex α) := ∀ w s cap, r.Terminates w s cap
+def AllTerminates (r : Regex α) := ∀ w s cap, r.Terminates w s cap
 
-theorem alwaysTerminates_bot : [/⊥/].AlwaysTerminates (α := α) :=
+theorem allTerminates_bot : [/⊥/].AllTerminates (α := α) :=
   fun _ _ _ ↦ terminates_bot
 
-theorem alwaysTerminates_empty : [//].AlwaysTerminates (α := α) :=
+theorem allTerminates_empty : [//].AllTerminates (α := α) :=
   fun _ _ _ ↦ terminates_empty
 
-theorem alwaysTerminates_unit {c : α} : [/c/].AlwaysTerminates (α := α) :=
+theorem allTerminates_unit {c : α} : [/c/].AllTerminates (α := α) :=
   fun _ _ _ ↦ terminates_unit
 
-theorem alwaysTerminates_concat {q r : Regex α}
-    (qt : q.AlwaysTerminates) (rt : r.AlwaysTerminates)
-    : [/⟨q⟩ ⟨r⟩/].AlwaysTerminates (α := α) :=
+theorem allTerminates_concat {q r : Regex α}
+    (qt : q.AllTerminates) (rt : r.AllTerminates)
+    : [/⟨q⟩ ⟨r⟩/].AllTerminates (α := α) :=
   fun w s cap ↦ terminates_concat.mpr ⟨qt w s cap, fun mat _ ↦ rt w mat.1 mat.2⟩
 
-theorem alwaysTerminates_or {q r : Regex α}
-    (qt : q.AlwaysTerminates) (rt : r.AlwaysTerminates)
-    : [/⟨q⟩ | ⟨r⟩/].AlwaysTerminates (α := α) :=
+theorem allTerminates_or {q r : Regex α}
+    (qt : q.AllTerminates) (rt : r.AllTerminates)
+    : [/⟨q⟩ | ⟨r⟩/].AllTerminates (α := α) :=
   fun w s cap ↦ terminates_or.mpr ⟨qt w s cap, rt w s cap⟩
 
-theorem alwaysTerminates_or_comm {q r : Regex α}
-    : [/⟨q⟩ | ⟨r⟩/].AlwaysTerminates ↔ [/⟨r⟩ | ⟨q⟩/].AlwaysTerminates := by
-  simp only [AlwaysTerminates, terminates_or_comm (q := q)]
+theorem allTerminates_or_comm {q r : Regex α}
+    : [/⟨q⟩ | ⟨r⟩/].AllTerminates ↔ [/⟨r⟩ | ⟨q⟩/].AllTerminates := by
+  simp only [AllTerminates, terminates_or_comm (q := q)]
 
-theorem alwaysTerminates_filterEmpty {e : Bool} {r : Regex α}
-    (rt : r.AlwaysTerminates)
-    : [/⟨r⟩ ‹e›ε/].AlwaysTerminates (α := α) :=
+theorem allTerminates_filterEmpty {e : Bool} {r : Regex α}
+    (rt : r.AllTerminates)
+    : [/⟨r⟩ ‹e›ε/].AllTerminates (α := α) :=
   fun w s cap ↦ terminates_filterEmpty.mpr (rt w s cap)
 
-theorem alwaysTerminates_star {t : StarType} {r : Regex α}
-    (rt : r.AlwaysTerminates)
-    : [/⟨r⟩*‹t›/].AlwaysTerminates (α := α) :=
+theorem allTerminates_star {t : StarType} {r : Regex α}
+    (rt : r.AllTerminates)
+    : [/⟨r⟩*‹t›/].AllTerminates (α := α) :=
   fun w _ _ ↦ terminates_star_of_forall fun s' _ cap' ↦ rt w s' cap'
 
-theorem alwaysTerminates_star_greedy_iff_lazy {r : Regex α}
-    : [/⟨r⟩*/].AlwaysTerminates ↔ [/⟨r⟩*?/].AlwaysTerminates := by
-  simp only [AlwaysTerminates, terminates_star_greedy_iff_lazy]
+theorem allTerminates_star_greedy_iff_lazy {r : Regex α}
+    : [/⟨r⟩*/].AllTerminates ↔ [/⟨r⟩*?/].AllTerminates := by
+  simp only [AllTerminates, terminates_star_greedy_iff_lazy]
 
-theorem alwaysTerminates_start : [/⊢/].AlwaysTerminates (α := α) :=
+theorem allTerminates_start : [/⊢/].AllTerminates (α := α) :=
   fun _ _ _ ↦ terminates_start
 
-theorem alwaysTerminates_end' : [/⊣/].AlwaysTerminates (α := α) :=
+theorem allTerminates_end' : [/⊣/].AllTerminates (α := α) :=
   fun _ _ _ ↦ terminates_end'
 
-theorem alwaysTerminates_capture {n : ℕ} {r : Regex α}
-    (rt : r.AlwaysTerminates)
-    : [/(‹n› ⟨r⟩)/].AlwaysTerminates (α := α) :=
+theorem allTerminates_capture {n : ℕ} {r : Regex α}
+    (rt : r.AllTerminates)
+    : [/(‹n› ⟨r⟩)/].AllTerminates (α := α) :=
   fun w s cap ↦ terminates_capture.mpr (rt w s cap)
 
-theorem alwaysTerminates_backref {d : BackrefDefault} {n : ℕ}
-    : [/\‹d›n/].AlwaysTerminates (α := α) := fun _ _ _ ↦ terminates_backref
+theorem allTerminates_backref {d : BackrefDefault} {n : ℕ}
+    : [/\‹d›n/].AllTerminates (α := α) := fun _ _ _ ↦ terminates_backref
 
 /-- A class of regexes that can be proven to always terminate -/
-inductive classTerminates : Regex α → Prop where
-  | bot : classTerminates bot
-  | empty : classTerminates empty
-  | unit c : classTerminates (unit c)
-  | concat q r : classTerminates q → classTerminates r → classTerminates (concat q r)
-  | or q r : classTerminates q → classTerminates r → classTerminates (or q r)
-  | filterEmpty e r : classTerminates r → classTerminates (filterEmpty e r)
-  | star t r : classTerminates r → classTerminates (star t r)
-  | start : classTerminates start
-  | end' : classTerminates end'
-  | capture n r : classTerminates r → classTerminates (capture n r)
-  | backref d n : classTerminates (backref d n)
+inductive CTerminates : Regex α → Prop where
+  | bot : CTerminates bot
+  | empty : CTerminates empty
+  | unit c : CTerminates (unit c)
+  | concat q r : CTerminates q → CTerminates r → CTerminates (concat q r)
+  | or q r : CTerminates q → CTerminates r → CTerminates (or q r)
+  | filterEmpty e r : CTerminates r → CTerminates (filterEmpty e r)
+  | star t r : CTerminates r → CTerminates (star t r)
+  | start : CTerminates start
+  | end' : CTerminates end'
+  | capture n r : CTerminates r → CTerminates (capture n r)
+  | backref d n : CTerminates (backref d n)
 
-/-- Rexeges constructed out of just ones in `classTerminates` always terminate -/
-theorem alwaysTerminates_classTerminates {r : Regex α} (hr : r.classTerminates)
-    : r.AlwaysTerminates := by
-  dsimp [AlwaysTerminates]
+/-- Rexeges constructed out of just ones in `cTerminates` always terminate -/
+theorem CTerminates.allTerminates {r : Regex α} (hr : r.CTerminates)
+    : r.AllTerminates := by
+  dsimp [AllTerminates]
   induction hr with
   | bot => termination
   | empty => termination
